src/named/Elab.v
@@ -6,70 +6,281 @@ Import ListNotations.
 Open Scope string.
 Open Scope list.
 From Utils Require Import Utils.
-From Named Require Import Exp ARule.
+From Named Require Import Core.
 (*TODO: why does this generate warnings?*)
-Import Exp.Notations.
-Import ARule.Notations.
-  
+Import Core.Notations.
+
+
+
 Section TermsAndRules.
-  Context (l' : lang).
+  Context (l : lang).
 
-  (* Assumes that the inputs are well-formed in the appropriate settings*)
-  Inductive elab_term : exp -> exp -> Prop :=
-  | elab_var x : elab_term (var x) (var x)
-  | elab_con n s s' c' args t
-    : In (n, (term_rule c' args t)) l' ->
-      elab_args args s (map fst c') s' ->
-      elab_term (con n s) (con n s')
-  with elab_args : list string -> list exp -> list string -> list exp -> Prop :=
-  | elab_args_nil : elab_args [] [] [] []
-  | elab_args_cons_ex e e' s s' n args args'
-    : elab_term e e' ->
-      elab_args args s args' s' ->
-      elab_args (n::args) (e::s) (n::args') (e'::s')
-  | elab_args_cons_im e e' s s' n args args'
-    : elab_term e e' ->
-      elab_args args s args' s' ->
-      elab_args args s (n::args') (e'::s').
-
-  Inductive elab_sort : sort -> sort -> Prop :=
-  | elab_scon n s s' c' args
-    : In (n, (sort_rule c' args)) l' ->
-      elab_args args s (map fst c') s' ->
-      elab_sort (scon n s) (scon n s').
+  (*All assume wf_lang.
+    All ctxs (other than in wf_ctx) are assumed to satisfy wf_ctx.
+    Judgments whose assumptions take ctxs must ensure they are wf.
+    Sorts are not assumed to be wf; the term judgments should guarantee
+    that their sorts are wf.
+   *)
   
-  Definition elab_subst : subst -> subst -> Prop :=
-    List.Forall2 (fun '(n,t) '(n',t') => n = n' /\ elab_term t t').
+ Inductive elab_term : ctx -> exp -> exp -> sort -> Prop :=
+  | elab_term_by : forall c n s es args c' t,
+      In (n, term_rule c' args t) l ->
+      elab_args c s args es c' ->
+      elab_term c (con n s) (con n es) t[/(with_names_from c' es)/]
+  | elab_term_conv : forall c e ee t t',
+      elab_term c e  ee t ->
+      eq_sort l c t t' ->
+      elab_term c e ee t'
+  | elab_term_var : forall c n t,
+      In (n, t) c ->
+      elab_term c (var n) (var n) t
+  with elab_args : ctx -> list exp -> list string -> list exp -> ctx -> Prop :=
+  | elab_args_nil : forall c, elab_args c [] [] [] []
+  | elab_args_cons_ex : forall c s args es c' name e ee t,
+      elab_term c e ee t[/with_names_from c' es/] ->
+      (* these arguments are last so that proof search unifies existentials
+       from the other arguments first*)
+      elab_args c s args es c' ->
+      elab_args c (e::s) (name::args) (ee::es) ((name,t)::c')
+  | elab_args_cons_im : forall c s args es c' name ee t,
+      elab_args c s args es c' ->
+      (* these arguments are last so that proof search unifies existentials
+       from the other arguments first*)
+      wf_term l c ee t[/with_names_from c' es/] ->
+      elab_args c s args (ee::es) ((name,t)::c')
+  with elab_sort : ctx -> sort -> sort -> Prop :=
+  | elab_sort_by : forall c n s args es c',
+      In (n, (sort_rule c' args)) l ->
+      elab_args c s args es c' ->
+      elab_sort c (scon n s) (scon n es)
+  with elab_ctx : ctx -> ctx-> Prop :=
+  | elab_ctx_nil : elab_ctx [] []
+  | elab_ctx_cons : forall name c ec v ev,
+      fresh name c ->
+      elab_ctx c ec ->
+      elab_sort ec v ev ->
+      elab_ctx ((name,v)::c) ((name,ev)::ec).
 
-  Definition elab_ctx : ctx -> ctx -> Prop :=
-    List.Forall2 (fun '(n,t) '(n',t') => n = n' /\ elab_sort t t').
+ 
+ Hint Constructors elab_sort elab_term elab_args elab_ctx : lang_core.
+ 
+ Scheme elab_sort_ind' := Minimality for elab_sort Sort Prop
+   with elab_term_ind' := Minimality for elab_term Sort Prop
+   with elab_args_ind' := Minimality for elab_args Sort Prop
+   with elab_ctx_ind' := Minimality for elab_ctx Sort Prop.
+ Combined Scheme elab_ind
+          from  elab_sort_ind', elab_term_ind', elab_args_ind', elab_ctx_ind'.
 
-  Variant elab_rule : rule -> rule -> Prop :=
-  | elab_sort_rule : forall c c' args,
-      elab_ctx c c' ->
-      elab_rule (sort_rule c args) (sort_rule c' args)
-  | elab_term_rule : forall c c' args t t',
-      elab_ctx c c' ->
-      elab_sort t t' ->
-      elab_rule (term_rule c args t) (term_rule c' args t')
-  | elab_le_sort_rule : forall c c' t1 t2 t1' t2',
-      elab_ctx c c' ->
-      elab_sort t1 t1' ->
-      elab_sort t2 t2' ->
-      elab_rule (sort_eq_rule c t1 t2) (sort_eq_rule c' t1' t2')
-  | elab_le_term_rule : forall c c' e1 e1' e2 e2' t t',
-      elab_ctx c c' ->
-      elab_sort t t' ->
-      elab_term e1 e1' ->
-      elab_term e2 e2' ->
-      elab_rule (term_eq_rule c e1 e2 t) (term_eq_rule c' e1' e2' t').
+ Lemma elab_ctx_preserves_fresh c ec n
+   : elab_ctx c ec ->
+     fresh n c ->
+     fresh n ec.
+ Proof.
+   induction 1; basic_goal_prep; basic_core_crush.
+ Qed.
+ Hint Resolve elab_ctx_preserves_fresh : lang_core.
+ 
+ Local Lemma elab_implies_wf
+   : (forall c t et,
+         elab_sort c t et ->
+         wf_sort l c et)
+     /\ (forall c e ee t,
+            elab_term c e ee t ->
+            wf_term l c ee t)
+     /\ (forall c s args es c',
+            elab_args c s args es c' ->
+            wf_args l c es c')
+     /\ (forall c ec,
+            elab_ctx c ec ->
+            wf_ctx l ec).
+ Proof using.
+   apply elab_ind; basic_goal_prep; basic_core_crush.
+ Qed.
+
+ Definition elab_sort_implies_wf := proj1 elab_implies_wf.
+ Hint Resolve elab_sort_implies_wf : lang_core.
+
+ Definition elab_term_implies_wf := proj1 (proj2 elab_implies_wf).
+ Hint Resolve elab_term_implies_wf : lang_core.
+
+ Definition elab_args_implies_wf := proj1 (proj2 (proj2 elab_implies_wf)).
+ Hint Resolve elab_args_implies_wf : lang_core.
+
+ Definition elab_ctx_implies_wf := proj2 (proj2 (proj2 elab_implies_wf)).
+ Hint Resolve elab_ctx_implies_wf : lang_core.
+
+
+ Variant elab_rule : rule -> rule -> Prop :=
+ | elab_sort_rule : forall c ec args,
+     elab_ctx c ec ->
+     sublist args (map fst ec) ->
+     elab_rule (sort_rule c args) (sort_rule ec args)
+ | elab_term_rule : forall c ec args t et,
+     elab_ctx c ec ->
+     elab_sort ec t et ->
+     sublist args (map fst ec) ->
+     elab_rule (term_rule c args t) (term_rule ec args et)
+ | eq_sort_rule : forall c ec t1 et1 t2 et2,
+     elab_ctx c ec ->
+     elab_sort ec t1 et1 ->
+     elab_sort ec t2 et2 ->
+     elab_rule (sort_eq_rule c t1 t2) (sort_eq_rule ec et1 et2)
+ | eq_term_rule : forall c ec e1 ee1 e2 ee2 t et,
+     elab_ctx c ec ->
+     elab_sort ec t et ->
+     elab_term ec e1 ee1 et ->
+     elab_term ec e2 ee2 et ->
+     elab_rule (term_eq_rule c e1 e2 t) (term_eq_rule ec ee1 ee2 et).
+ 
+ Lemma elab_rule_implies_wf r er
+   : elab_rule r er ->
+     wf_rule l er.
+ Proof using.
+   destruct 1; basic_goal_prep; basic_core_crush.
+ Qed.
+
+(* TODO: do I need this?
+  Inductive elab_subst c : subst -> ctx -> Prop :=
+  | elab_subst_nil : elab_subst c [] []
+  | elab_subst_cons : forall s c' name e t,
+      (* assumed because the output ctx is wf: fresh name c' ->*)
+      elab_subst c s c' ->
+      elab_term c e t[/s/] ->
+      elab_subst c ((name,e)::s) ((name,t)::c').
+ *)
+ 
 End TermsAndRules.
-  
+
 Inductive elab_lang : lang -> lang -> Prop :=
 | elab_lang_nil : elab_lang [] []
-| elab_lang_cons n l l' r r'
-  : elab_lang l l' ->
-    elab_rule l' r r' ->
-    elab_lang ((n,r)::l) ((n,r')::l').
+| elab_lang_cons : forall l el n r er,
+    fresh n l ->
+    elab_lang l el ->
+    elab_rule el r er ->
+    elab_lang ((n,r)::l) ((n,er)::el).
 
-Hint Constructors elab_lang elab_rule elab_sort List.Forall2 elab_args elab_term : exp.
+
+Lemma elab_lang_preserves_fresh c ec n
+  : elab_lang c ec ->
+    fresh n c ->
+    fresh n ec.
+Proof.
+  induction 1; basic_goal_prep; basic_core_crush.
+Qed.
+Hint Resolve elab_lang_preserves_fresh : lang_core.
+
+
+Local Hint Resolve elab_rule_implies_wf : lang_core.
+Lemma elab_lang_implies_wf l el
+  : elab_lang l el ->
+    wf_lang el.
+Proof using.
+  induction 1; basic_goal_prep; basic_core_crush.
+Qed.
+#[export] Hint Resolve elab_lang_implies_wf : lang_core.
+
+#[export] Hint Constructors elab_sort elab_term elab_args elab_ctx
+ elab_rule elab_lang : lang_core.
+
+
+
+Lemma elab_lang_cons_nth_tail n l el name r er el'
+  : nth_error l n = Some (name,r) ->
+    nth_tail n el = (name, er)::el' ->
+    fresh name (nth_tail (S n) l) ->
+    elab_lang (nth_tail (S n) l) (nth_tail (S n) el) ->
+    elab_rule (nth_tail (S n) el) r er ->
+    elab_lang (nth_tail n l) (nth_tail n el).
+Proof.
+  revert el n el'.
+  induction l; destruct el; basic_goal_prep; basic_core_crush.
+  {
+    apply nth_error_In in H.
+    basic_utils_crush.
+  }
+  {
+    destruct n.
+    {
+      rewrite <-!as_nth_tail in *.
+      basic_goal_prep;
+        basic_core_crush.
+    }
+    {
+      rewrite !nth_tail_S_cons in *.
+      eauto.
+    }
+  }
+Qed.
+
+Ltac break_down_elab_lang :=
+  repeat ((eapply elab_lang_cons_nth_tail; [compute; reflexivity | compute; reflexivity| apply use_compute_fresh; compute; reflexivity | ..]));
+  [compute; apply elab_lang_nil|..].
+
+
+Lemma elab_term_by' l c n (s es : list exp) args c' t t'
+  : In (n, term_rule c' args t') l ->
+    elab_args l c s args es c' ->
+    t = t' [/with_names_from c' es /] ->
+    elab_term l c (con n s) (con n es) t.
+Proof.
+  intros; subst; eauto with lang_core.
+Qed.
+
+Lemma wf_term_by' l c n (es : list exp) args c' t t'
+  : In (n, term_rule c' args t') l ->
+    wf_args l c es c' ->
+    t = t' [/with_names_from c' es /] ->
+    wf_term l c (con n es) t.
+Proof.
+  intros; subst; eauto with lang_core.
+Qed.
+
+
+Lemma elab_args_cons_ex' l c s args es c' name e ee t
+  : len_eq es c' -> (*used to instantiate es with conses*)
+    elab_term l c e ee t[/with_names_from c' es/] ->
+    (* these arguments are last so that proof search unifies existentials
+       from the other arguments first*)
+    elab_args l c s args es c' ->
+    elab_args l c (e::s) (name::args) (ee::es) ((name,t)::c').
+Proof.
+  eauto with lang_core.
+Qed.
+
+Local Ltac t :=
+  match goal with
+  | [|- fresh _ _ ]=> apply use_compute_fresh; compute; reflexivity
+  | [|- sublist _ _ ]=> apply (use_compute_sublist string_dec); compute; reflexivity
+  | [|- In _ _ ]=> apply named_list_lookup_err_in; compute; reflexivity
+  | [|- len_eq _ _] => econstructor
+  | [|-elab_sort _ _ _ _] => eapply elab_sort_by
+  | [|-elab_ctx _ _ _] => econstructor
+  | [|-elab_args _ _ _ _ _ _] => eapply elab_args_cons_ex' || econstructor
+  | [|-elab_term _ _ _ _ _] => eapply elab_term_var || eapply elab_term_by'
+  | [|-wf_term _ _ _ _] => shelve
+  | [|-elab_rule _ _ _] => econstructor
+  | [|- _ = _] => compute; reflexivity
+  end.
+
+Ltac auto_elab :=
+  match goal with
+  | [|- elab_lang ?l ?el] =>
+  rewrite (as_nth_tail l);
+  rewrite (as_nth_tail el);
+  break_down_elab_lang;
+  solve[repeat t]
+  end.
+
+
+Local Ltac t' :=
+  match goal with
+  | [|- fresh _ _ ]=> apply use_compute_fresh; compute; reflexivity
+  | [|- sublist _ _ ]=> apply (use_compute_sublist string_dec); compute; reflexivity
+  | [|- In _ _ ]=> apply named_list_lookup_err_in; compute; reflexivity
+  | [|- wf_term _ _ _ _] =>  eapply wf_term_var || eapply wf_term_by'
+  | [|-wf_args _ _ _ _] => econstructor
+  | [|- _ = _] => compute; reflexivity
+  end.
+
+Ltac cleanup_auto_elab :=
+  solve [ repeat t'].
